

Lecture# 18 (Derivative of vector valued function)

Thursday, November 6, 2025 11:11 AM

Derivative of Position = velocity

$$\vec{r}(t) = \langle f_1(t), f_2(t), f_3(t) \rangle$$

$$\frac{d\vec{r}}{dt} = \langle f_1'(t), f_2'(t), f_3'(t) \rangle$$

Rule

$$(1) \frac{d}{dt}(c \vec{r}(t)) = c \cdot \frac{d}{dt} \vec{r}(t) = c \vec{r}'(t)$$

$$(2) \frac{d}{dt}(u(t) \vec{r}(t)) = u \cdot \vec{r}'(t) + u' \vec{r}(t) \quad \text{Product Rule}$$

$$(3) \frac{d}{dt}(u(t) \cdot \vec{r}(t)) = u(t) \cdot \vec{r}'(t) + u'(t) \cdot \vec{r}(t) \quad \text{dot Product}$$

$$(4) \frac{d}{dt}(u(t) \times \vec{r}(t)) = u(t) \times \vec{r}'(t) + u'(t) \times \vec{r}(t) \quad \text{cross Product}$$

Properties of the Derivative of Vector-Valued Functions

Let \mathbf{r} and \mathbf{u} be differentiable vector-valued functions of t , let f be a differentiable real-valued function of t , a scalar.

- | | | |
|------|--|--------------------|
| i. | $\frac{d}{dt}[c\mathbf{r}(t)] = c\mathbf{r}'(t)$ | Scalar multiple |
| ii. | $\frac{d}{dt}[\mathbf{r}(t) \pm \mathbf{u}(t)] = \mathbf{r}'(t) \pm \mathbf{u}'(t)$ | Sum and difference |
| iii. | $\frac{d}{dt}[f(t)\mathbf{u}(t)] = f'(t)\mathbf{u}(t) + f(t)\mathbf{u}'(t)$ | Scalar product |
| iv. | $\frac{d}{dt}[\mathbf{r}(t) \cdot \mathbf{u}(t)] = \mathbf{r}'(t) \cdot \mathbf{u}(t) + \mathbf{r}(t) \cdot \mathbf{u}'(t)$ | Dot product |
| v. | $\frac{d}{dt}[\mathbf{r}(t) \times \mathbf{u}(t)] = \mathbf{r}'(t) \times \mathbf{u}(t) + \mathbf{r}(t) \times \mathbf{u}'(t)$ | Cross product |
| vi. | $\frac{d}{dt}[\mathbf{r}(f(t))]$ $= \mathbf{r}'(f(t)) \cdot f'(t)$ | Chain rule |
| vii. | If $\mathbf{r}(t) \cdot \mathbf{r}(t) = c$, then $\mathbf{r}(t) \cdot \mathbf{r}'(t) = 0$. | |

$$(x^2 + 3x)^5 = 5(x^2 + 3x)^4(2x + 3)$$

- $\frac{d}{dt}[\sin(at)] = a \times \cos(at)$ $\frac{d}{dt}(\sin(f(t))) = \cos(f(t)) \cdot f'(t)$
- $\frac{d}{dt}[\cos(at)] = -a \times \sin(at)$

a. We have $\mathbf{r}'(t) = 6\mathbf{i} + (8t+2)\mathbf{j} + 5\mathbf{k}$ and $\mathbf{u}'(t) = 2t\mathbf{i} + 2\mathbf{j} + (3t^2-3)\mathbf{k}$. Therefore, according to property iv.:

$$\frac{d}{dt}[\mathbf{r}(t) \cdot \mathbf{u}(t)] = \mathbf{r}'(t) \cdot \mathbf{u}(t) + \mathbf{r}(t) \cdot \mathbf{u}'(t)$$

$$\begin{aligned} &= (6\mathbf{i} + (8t+2)\mathbf{j} + 5\mathbf{k}) \cdot ((t^2-3)\mathbf{i} + (2t+4)\mathbf{j} + (t^3-3t)\mathbf{k}) \\ &\quad + ((6t+8)\mathbf{i} + (4t^2+2t-3)\mathbf{j} + 5t\mathbf{k}) \cdot (2t\mathbf{i} + 2\mathbf{j} + (3t^2-3)\mathbf{k}) \\ &= 6(t^2-3) + (8t+2)(2t+4) + 5(t^3-3t) \\ &\quad + 2t(6t+8) + 2(4t^2+2t-3) + 5t(3t^2-3) \\ &= 20t^3 + 42t^2 + 26t - 16. \end{aligned}$$

$$\begin{pmatrix} 6 \\ 8t+2 \\ 5t \end{pmatrix}$$

$$\begin{cases} \mathbf{r}(t) = (6t+8)\mathbf{i} + (4t^2+2t-3)\mathbf{j} + 5t\mathbf{k} & ; \mathbf{r}' = 6\mathbf{i} + (8t+2)\mathbf{j} + 5\mathbf{k} \\ \mathbf{u}(t) = (t^2-3)\mathbf{i} + (2t+4)\mathbf{j} + (t^3-3t)\mathbf{k}, & \mathbf{u}' = 2t\mathbf{i} + 2\mathbf{j} + (3t^2-3)\mathbf{k} \end{cases}$$

$$\frac{d}{dt}(\vec{r} \cdot \vec{u}) = \vec{r} \cdot \vec{u}' + \vec{r}' \cdot \vec{u}$$

do your self 😊

$$\vec{r} \cdot \vec{u}' = \begin{pmatrix} 6t+8 \\ 4t^2+2t-3 \\ 5t \end{pmatrix} \cdot \begin{pmatrix} 2t \\ 2 \\ 3t^2-3 \end{pmatrix}$$

$$\begin{aligned} &= 2t(6t+8) + 2(4t^2+2t-3) + 5t(3t^2-3) \\ &= 12t^2 + 16t + 8t^2 + 4t - 6 + 15t^3 - 15t \\ &= 15t^3 + 20t^2 + 5t - 6 \end{aligned}$$

$$\frac{d}{dt}(\vec{u} \times \vec{r}) = \boxed{\vec{u} \times \vec{r}'} + \boxed{\vec{u}' \times \vec{r}} \quad \text{property of derivative}$$

① Direct

$$\text{Calculator } \vec{u} \times \vec{r} = \begin{vmatrix} \vec{i} & \vec{j} & \vec{k} \\ u_1 & u_2 & u_3 \\ r_1 & r_2 & r_3 \end{vmatrix}$$

$$= \vec{i}(\underline{u_2 r_3 - u_3 r_2}) - \vec{j}(\underline{u_1 r_3 - r_1 u_3}) + \vec{k}(\underline{u_1 r_2 - r_1 u_2})$$

$$\frac{d}{dt}(\vec{u} \times \vec{r})$$